lemma_4_1 verifies

src/dvspec/dafny/att_spec_proofs/inv.dfy
@@ -966,8 +966,26 @@ module Att_Inv_With_Empty_Initial_Attestation_Slashing_DB
                 vp == (ad: AttestationData) => consensus_is_valid_attestation_data(attestation_slashing_db, ad, attestation_duty)
     }
 
-
     predicate pred_4_1_g_b(dvn: DVState)
+    {
+        forall hn, s1: nat, s2: nat, vp, attestation_duty, attestation_slashing_db |
+            && hn in dvn.honest_nodes_states.Keys
+            && s1 < s2
+            && hn in dvn.consensus_on_attestation_data[s1].honest_nodes_validity_functions.Keys
+            && hn in dvn.consensus_on_attestation_data[s2].honest_nodes_validity_functions.Keys
+            && vp in dvn.consensus_on_attestation_data[s2].honest_nodes_validity_functions[hn]
+            && vp == (ad: AttestationData) => consensus_is_valid_attestation_data(attestation_slashing_db, ad, attestation_duty)
+            ::
+            && dvn.consensus_on_attestation_data[s1].decided_value.isPresent()
+            && var decided_a_data := dvn.consensus_on_attestation_data[s1].decided_value.safe_get();
+            && var sdba := SlashingDBAttestation(
+                                            source_epoch := decided_a_data.source.epoch,
+                                            target_epoch := decided_a_data.target.epoch,
+                                            signing_root := Some(hash_tree_root(decided_a_data)));
+            && sdba in attestation_slashing_db
+    }    
+
+    predicate pred_4_1_g_b_thanh_hai(dvn: DVState)
     {
         forall hn, s1: nat, s2: nat, vp |
             && hn in dvn.honest_nodes_states.Keys
@@ -989,7 +1007,6 @@ module Att_Inv_With_Empty_Initial_Attestation_Slashing_DB
                                             signing_root := Some(hash_tree_root(decided_a_data)));
             && sdba in db2
     }    
-
 
     predicate inv43_body(dvn: DVState, hn: BLSPubkey, s: Slot)
     requires is_honest_node(dvn, hn)
